simplify conditional counter: get rid of histories; instead of heap metadata for ABA protection
Also needs a new token and splitting ownership of the "main" protocol location.

theories/logatom/cinc.v
@@ -1,4 +1,4 @@
-From iris.algebra Require Import excl auth agree frac list cmra.
+From iris.algebra Require Import excl auth agree frac list cmra csum.
 From iris.base_logic.lib Require Export invariants.
 From iris.program_logic Require Export atomic.
 From iris.proofmode Require Import tactics.
@@ -89,244 +89,20 @@ Definition cinc : val :=
 
 (** ** Proof setup *)
 
-(** To represent histories of allocated locations, we need some helper lemmas
-    about suffixes on lists. *)
-Section suffixes.
-
-  Lemma suffix_trans (h1 h2 h3 : list loc) :
-    h1 `suffix_of` h2 →
-    h2 `suffix_of` h3 →
-    h1 `suffix_of` h3.
-  Proof.
-    intros [? ->] [? ->]. rewrite app_assoc. by eexists.
-  Qed.
-
-  Lemma suffix_eq (h1 h2 : list loc) :
-    h1 `suffix_of` h2 →
-    h2 `suffix_of` h1 →
-    h1 = h2.
-  Proof.
-    intros [xs ->] [ys Heq]. rewrite <- app_nil_l in Heq at 1. rewrite app_assoc in Heq.
-    apply app_inv_tail, eq_sym in Heq. by apply app_eq_nil in Heq as [_ ->].
-  Qed.
-
-  Lemma suffix_in (h1 h2 : list loc) l :
-    h1 `suffix_of` h2 →
-    In l h1 →
-    In l h2.
-  Proof.
-    destruct h1 as [|y ys]; first done.
-    intros Hs Hin. destruct Hs as [l2' ->]. apply in_or_app. by right.
-  Qed.
-
-  Lemma suffix_in_head (h1 h2 : list loc) l :
-    h1 `suffix_of` h2 →
-    Some l = head h1 →
-    In l h2.
-  Proof.
-    destruct h1 as [|y ys]; first done.
-    intros Hs [=->]. eapply suffix_in; first done. apply in_eq.
-  Qed.
-
-  (** A helper lemma that will come up in the proof of [complete] *)
-  Lemma nodup_suffix_contradiction (l1 l2 l3 : loc) (H1 H2 H3 : list loc) :
-    Some l1 = hd_error H1 →
-    Some l2 = hd_error H2 →
-    Some l3 = hd_error H3 →
-    In l3 H1 →
-    H1 `suffix_of` H2 →
-    H2 `suffix_of` H3 →
-    l2 ≠ l3 →
-    NoDup H3 →
-    False.
-  Proof.
-    intros Heq Heq' Heq'' Hin Hs Hs' Hn Hd.
-    destruct Hs' as [xs ->]. destruct Hs as [ys ->]. destruct (in_split _ _ Hin) as (x & y & ->).
-    do 2 rewrite app_assoc in Hd. apply NoDup_remove_2 in Hd.
-    (* xs, ys, and x must be empty *)
-    destruct xs as [|x' xs]; last first.
-    { simpl in *. inversion Heq''. subst.
-      contradict Hd. by left. }
-    destruct ys as [|y' ys]; last first.
-    { simpl in *. inversion Heq''; subst.
-      contradict Hd. by left. }
-    destruct x as [|z' zs]; last first.
-    { simpl in *. inversion Heq''; subst.
-      contradict Hd. by left. }
-    simpl in *. inversion Heq'; done.
-  Qed.
-
-End suffixes.
-
-(** Resource algebra for histories *)
-Section histories.
-
-  Inductive hist :=
-  | histv (h : list loc) : hist
-  | histbot : hist.
-
-  Inductive hist_equiv : Equiv hist :=
-  | Hist_equiv h1 h2 : h1 = h2 → h1 ≡ h2.
-
-  Existing Instance hist_equiv.
-
-  Instance hist_equiv_Equivalence : @Equivalence hist equiv.
-  Proof.
-    split.
-    - move => [|]; by constructor.
-    - move => [?|] []; inversion 1; subst; by constructor.
-    - move => [?|] [] [];
-               inversion 1; inversion 1; subst; by constructor.
-  Qed.
-
-  Canonical Structure histC : ofeT := discreteC hist.
-
-  Instance hist_valid : Valid hist :=
-    λ x, match x with histv _ => True | histbot => False end.
-
-  Instance hist_op : Op hist := λ h1 h2,
-                                match h1, h2 with
-                                | histv h1', histv h2' =>
-                                  if decide (h1' `suffix_of` h2')
-                                  then h2
-                                  else if decide (h2' `suffix_of` h1')
-                                       then h1
-                                       else histbot
-                                | _, _ =>
-                                  histbot
-                                end.
-
-  Arguments op _ _ !_ !_ /.
-
-  Instance hist_PCore : PCore hist := Some.
-
-  Global Instance hist_op_comm: Comm equiv hist_op.
-  Proof.
-    intros [h1|] [h2|]; auto. simpl.
-    case_decide as H1; [case_decide as H2|auto]; last auto.
-    constructor. destruct H1. subst.  destruct H2.
-    rewrite <- app_nil_l in H at 1. rewrite app_assoc in H.
-      by apply app_inv_tail, eq_sym, app_eq_nil in H as [-> ->].
-  Qed.
-
-  Global Instance hist_op_idemp : IdemP eq hist_op.
-  Proof. intros [|]; [by simpl; rewrite decide_True|auto]. Qed.
-
-  Lemma hist_op_l h1 h2 (Le: h1 `suffix_of` h2) :
-    histv h1 ⋅ histv h2 = histv h2.
-  Proof. simpl. case_decide; done. Qed.
-
-  Lemma hist_op_r h1 h2 (Le: h1 `suffix_of` h2) :
-    histv h2 ⋅ histv h1 = histv h2.
-  Proof.
-    simpl. case_decide.
-    - f_equal. by apply suffix_eq.
-    - by case_decide.
-  Qed.
-
-  Global Instance hist_op_assoc: Assoc equiv (op: Op hist).
-  Proof.
-    intros [h1|] [h2|] [h3|]; eauto; simpl.
-    - repeat (case_decide; auto).
-      + rewrite !hist_op_l; auto. etrans; eauto.
-      + simpl. repeat case_decide; last done.
-        * destruct H as [xs ->]. destruct H2 as [ys [[k [->->]] | [k [->->]]]%app_eq_inv].
-          ** contradict H1. by apply suffix_app_r.
-          ** contradict H0. by apply suffix_app_r.
-        * contradict H1. by etrans.
-      + rewrite hist_op_l; [by rewrite hist_op_r|auto].
-      + rewrite !hist_op_r; auto. by etrans.
-      + simpl. rewrite !decide_False; auto.
-      + simpl. rewrite !decide_False; auto.
-      + simpl. case_decide.
-        * exfalso. apply H. by etrans.
-        * case_decide; last done. exfalso.
-          destruct H4 as [xs ->]. destruct H2 as [ys [[k [->->]] | [k [->->]]]%app_eq_inv].
-          ** contradict H0. by apply suffix_app_r.
-          ** contradict H. by apply suffix_app_r.
-    - simpl. repeat case_decide; auto.
-  Qed.
-
-  Lemma hist_included h1 h2 :
-    histv h1 ≼ histv h2 ↔ h1 `suffix_of` h2.
-  Proof.
-    split.
-    - move => [[?|]]; simpl; last by inversion 1.
-      case_decide.
-      * inversion 1. naive_solver.
-      * case_decide; inversion 1; naive_solver.
-    - intros. exists (histv h2). by rewrite hist_op_l.
-  Qed.
-
-  Lemma hist_valid_op h1 h2 :
-    ✓ (histv h1 ⋅ histv h2) → h1 `suffix_of` h2 ∨ h2 `suffix_of` h1.
-  Proof. simpl. case_decide; first by left. case_decide; [by right|done]. Qed.
-
-  Lemma hist_core_self (X: hist) : core X = X.
-  Proof. done. Qed.
-
-  Instance hist_unit : Unit hist := histv nil.
-
-  Definition hist_ra_mixin : RAMixin hist.
-  Proof.
-    apply ra_total_mixin; eauto.
-    - intros [?|] [?|] [?|]; auto; inversion 1; naive_solver.
-    - by destruct 1; constructor.
-    - destruct 1. naive_solver.
-    - apply hist_op_assoc.
-    - apply hist_op_comm.
-    - intros ?. by rewrite hist_core_self idemp_L.
-    - intros [|] [|]; simpl; done.
-  Qed.
-
-  Canonical Structure histR := discreteR hist hist_ra_mixin.
-
-  Global Instance hist_cmra_discrete : CmraDiscrete histR.
-  Proof. apply discrete_cmra_discrete. Qed.
-
-  Global Instance hist_core (h: hist) : CoreId h.
-  Proof.
-    rewrite /CoreId. reflexivity.
-  Qed.
-
-  Definition hist_ucmra_mixin : UcmraMixin hist.
-  Proof.
-    split; [done| |auto]. intros [|]; [simpl|done]. done.
-  Qed.
-
-  Lemma hist_local_update h1 X h2 :
-    h1 `suffix_of` h2 → (histv h1, X) ~l~> (histv h2, histv h2).
-  Proof.
-    intros Le. rewrite local_update_discrete.
-    move => [[h3|]|] /= ? Eq; split => //; last first; move : Eq.
-    - destruct X; by inversion 1.
-    - destruct X; rewrite /cmra_op /= => Eq;
-                                          repeat case_decide; auto; inversion Eq; subst; try naive_solver.
-      + constructor. inversion H1. subst. f_equal. by apply suffix_eq.
-      + constructor. inversion H2. subst. f_equal. apply suffix_eq; by etrans.
-      + inversion H3; subst. by apply (suffix_trans _ _ _ H0) in Le.
-  Qed.
-
-  Canonical Structure histUR := UcmraT hist hist_ucmra_mixin.
-
-End histories.
-
-Definition histListUR := optionUR $ prodR fracR $ agreeR $ listC locC.
-
-Definition historyUR := prodUR (authUR histListUR) (authUR histUR).
-Definition flagUR    := authR $ optionUR $ exclR boolC.
-Definition numUR     := authR $ optionUR $ exclR ZC.
-Definition tokenUR   := authR $ optionUR $ exclR valC.
+Definition flagUR     := authR $ optionUR $ exclR boolC.
+Definition numUR      := authR $ optionUR $ exclR ZC.
+Definition tokenUR    := exclR unitC.
+Definition one_shotUR := csumR (exclR unitC) (agreeR unitC).
 
 Class cincG Σ := ConditionalIncrementG {
-                     cinc_historyG :> inG Σ historyUR;
-                     cinc_flagG    :> inG Σ flagUR;
-                     cinc_numG     :> inG Σ numUR;
-                     cinc_tokenG   :> inG Σ tokenUR;
+                     cinc_flagG     :> inG Σ flagUR;
+                     cinc_numG      :> inG Σ numUR;
+                     cinc_tokenG    :> inG Σ tokenUR;
+                     cinc_one_shotG :> inG Σ one_shotUR;
                    }.
 
 Definition cincΣ : gFunctors :=
-  #[GFunctor historyUR; GFunctor flagUR; GFunctor numUR; GFunctor tokenUR].
+  #[GFunctor flagUR; GFunctor numUR; GFunctor tokenUR; GFunctor one_shotUR].
 
 Instance subG_cincΣ {Σ} : subG cincΣ Σ → cincG Σ.
 Proof. solve_inG. Qed.
@@ -338,84 +114,7 @@ Section conditional_counter.
   Local Definition stateN   := N .@ "state".
   Local Definition counterN := N .@ "counter".
 
-  Definition token : tokenUR :=
-    ● Excl' #().
-
-  Definition histList (H : list loc) (q : Qp) : histListUR :=
-    Some (q, to_agree H).
-
-  Definition half_history_frag (H : list loc) : historyUR :=
-    (◯ (histList H (1/2)%Qp), ◯ (histv H)).
-
-  Definition full_history_frag (H : list loc) : historyUR :=
-    (◯ (histList H 1%Qp), ◯ (histv H)).
-
-  Definition full_history_auth (H : list loc) : historyUR :=
-    (● (histList H 1%Qp), ● (histv H)).
-
-  Definition hist_snapshot H : historyUR :=
-    (◯ None, ◯ histv H).
-
-  Global Instance snapshot_persistent H γ_h : Persistent (own γ_h (hist_snapshot H)).
-  Proof.
-    apply own_core_persistent. rewrite /CoreId. done.
-  Qed.
-
-  (** Updating and synchronizing history RAs *)
-
-  Lemma sync_histories H1 H2 γ_h :
-    own γ_h (half_history_frag H1) -∗ own γ_h (half_history_frag H2) -∗ ⌜H1 = H2⌝.
-  Proof.
-    iIntros "H1 H2". iCombine "H1" "H2" as "H". iPoseProof (own_valid with "H") as "H".
-    iDestruct "H" as %H. iPureIntro. destruct H as [[_ Hl1%agree_op_inv] _].
-    by apply to_agree_inj, leibniz_equiv in Hl1.
-  Qed.
-
-  Lemma add_half_histories (H : list loc) γ_h :
-    own γ_h (half_history_frag H) -∗
-        own γ_h (half_history_frag H) -∗
-        own γ_h (full_history_frag H).
-  Proof.
-    iIntros "H1 H2". iCombine "H1" "H2" as "H". done.
-  Qed.
-
-  Lemma update_history H H' l γ_h :
-    own γ_h (full_history_auth H) -∗
-        own γ_h (half_history_frag H) -∗
-        own γ_h (half_history_frag H') ==∗
-        own γ_h (full_history_auth (l :: H)) ∗
-        own γ_h (half_history_frag (l :: H)) ∗
-        own γ_h (half_history_frag (l :: H)).
-  Proof.
-    iIntros "H● H1◯ H2◯". iDestruct (sync_histories with "H1◯ H2◯") as %<-.
-    iDestruct (add_half_histories with "H1◯ H2◯") as "H◯".
-    iCombine "H● H◯" as "H". rewrite -own_op -own_op.
-    iApply (own_update with "H"). apply prod_update.
-    - apply auth_update, option_local_update. rewrite pair_op frac_op' agree_idemp.
-      rewrite Qp_div_2. apply exclusive_local_update. by constructor.
-    - apply auth_update. simpl. rewrite hist_op_l; last done.
-        by apply hist_local_update, suffix_cons_r.
-  Qed.
-
-  Lemma sync_snapshot H1 H2 H2' γ_h :
-    own γ_h (full_history_auth H1) -∗ own γ_h (◯ H2', ◯ histv H2) -∗ ⌜H2 `suffix_of` H1⌝.
-  Proof.
-    iIntros "H● H◯". iCombine "H●" "H◯" as "H".
-      by iDestruct (own_valid with "H") as %[_ [Hs%hist_included _]%auth_both_valid].
-  Qed.
-
-  Lemma extract_snapshot H γ_h :
-     own γ_h (half_history_frag H) -∗ □ own γ_h (hist_snapshot H).
-   Proof.
-     iIntros "H".
-     iAssert (own γ_h (half_history_frag H) ∗ own γ_h (hist_snapshot H))%I with "[H]" as "[_ H2]".
-     { rewrite -own_op pair_op.
-       assert (◯ histList H (1 / 2) ⋅ ◯ None = ◯ (histList H (1 / 2) ⋅ None)) as Heq by apply auth_frag_op.
-       assert (◯ histv H ⋅ ◯ histv H = ◯ (histv H ⋅ histv H)) as Heq' by apply auth_frag_op.
-       rewrite Heq Heq' right_id. rewrite <- core_id_dup; first done. by rewrite /CoreId. }
-     rewrite intuitionistically_into_persistently.
-     by iApply persistent.
-   Qed.
+  (** Updating and synchronizing the counter and flag RAs *)
 
   Lemma sync_counter_values γ_n (n m : Z) :
     own γ_n (● Excl' n) -∗ own γ_n (◯ Excl' m) -∗ ⌜n = m⌝.
@@ -423,9 +122,6 @@ Section conditional_counter.
     iIntros "H● H◯". iCombine "H●" "H◯" as "H". iDestruct (own_valid with "H") as "H".
       by iDestruct "H" as %[H%Excl_included%leibniz_equiv _]%auth_both_valid.
   Qed.
-
-
-  (** Updating and synchronizing the counter and flag RAs *)
 
   Lemma sync_flag_values γ_n (b1 b2 : bool) :
     own γ_n (● Excl' b1) -∗ own γ_n (◯ Excl' b2) -∗ ⌜b1 = b2⌝.
@@ -448,8 +144,8 @@ Section conditional_counter.
     by apply auth_update, option_local_update, exclusive_local_update.
   Qed.
 
-  Definition counter_content (γs : gname * gname * gname) (c : bool * Z) :=
-    (own γs.1.2 (◯ Excl' c.1) ∗ own γs.2 (◯ Excl' c.2))%I.
+  Definition counter_content (γs : gname * gname) (c : bool * Z) :=
+    (own γs.1 (◯ Excl' c.1) ∗ own γs.2 (◯ Excl' c.2))%I.
 
 
   (** Definition of the invariant *)
@@ -474,55 +170,84 @@ Section conditional_counter.
     destruct l0; try by right. simpl in H. inversion H. by left.
   Qed.
 
+  (** Removing a #false does not change the result. *)
+  Lemma val_to_loc_pop_false vs (l : loc) :
+    val_to_some_loc ((#false, #l)::vs) = val_to_some_loc vs.
+  Proof. reflexivity. Qed.
+
   Inductive abstract_state : Set :=
   | injl : Z → abstract_state
   | injr : Z → proph_id → abstract_state.
 
-  Definition own_token γ_t := (own γ_t token)%I.
+  Definition state_to_val (s : abstract_state) : val :=
+    match s with
+    | injl n => InjLV #n
+    | injr n p => InjRV (#n,#p)
+    end.
 
-  Definition used_up l γ_h :=
-    (∃ H, □ own γ_h (hist_snapshot H) ∗ ⌜In l H ∧ Some l ≠ head H⌝)%I.
+  Global Instance state_to_val_inj : Inj (=) (=) state_to_val.
+  Proof.
+    intros [|] [|]; simpl; intros Hv; inversion_clear Hv; done.
+  Qed.
 
-  Definition not_done_state H l (γ_h : gname) :=
-    (own γ_h (half_history_frag H) ∗ ⌜Some l = head H⌝)%I.
+  Definition own_token γ := (own γ (Excl ()))%I.
 
-  Definition pending_state P (n : Z) vs l_ghost (γ_h γ_n : gname) :=
-    (P ∗ ⌜match val_to_some_loc vs with None => True | Some l => l = l_ghost end⌝ ∗ own γ_n (● Excl' n))%I.
+  Definition loc_token (l: loc) := (∃ γ, meta l N γ ∗ own_token γ)%I.
 
-  Definition accepted_state Q vs (l l_ghost : loc) (γ_h : gname) :=
-    (l_ghost ↦{1/2} - ∗ match val_to_some_loc vs with None => True | Some l => ⌜l = l_ghost⌝ ∗ Q end)%I.
+  Definition pending_state P (n : Z) (proph_winner : option loc) l_ghost_winner (γ_n : gname) :=
+    (P ∗ ⌜match proph_winner with None => True | Some l => l = l_ghost_winner end⌝ ∗ own γ_n (● Excl' n))%I.
 
-  Definition done_state Q (l l_ghost : loc) (γ_t γ_h  : gname) :=
-    ((Q ∨ own_token γ_t) ∗ l_ghost ↦ - ∗ used_up l γ_h)%I.
+  (* After the prophecy said we are going to win the race, we commit and run the AU,
+     switching from [pending] to [accepted]. *)
+  Definition accepted_state Q (proph_winner : option loc) (l_ghost_winner : loc) :=
+    (l_ghost_winner ↦{1/2} - ∗ match proph_winner with None => True | Some l => ⌜l = l_ghost_winner⌝ ∗ Q end)%I.
 
-  Definition state_inv P Q (p : proph_id) n l l_ghost H γ_h γ_n γ_t : iProp Σ :=
+  (* The same thread then wins the CAS and moves from [accepted] to [done].
+     Then, the [γ_t] token guards the transition to take out [Q].
+     Remember that the thread winning the CAS might be just helping.  The token
+     is owned by the thread whose request this is.
+     In this state, [l_ghost_winner] serves as a token to make sure that
+     only the CAS winner can transition to here, and [loc_token l] serves as a
+     "location" token to ensure there is no ABA going on. *)
+  Definition done_state Q (l l_ghost_winner : loc) (γ_t : gname) :=
+    ((Q ∨ own_token γ_t) ∗ l_ghost_winner ↦ - ∗ loc_token l)%I.
+
+  (* We always need the [proph] in here so that failing threads coming late can
+     always resolve their stuff.
+     Moreover, we need a way for anyone who has observed the [done] state to
+     prove that we will always remain [done]; that's what the one-shot token [γ_s] is for. *)
+  Definition state_inv P Q (p : proph_id) n (c_l l l_ghost_winner : loc) γ_n γ_t γ_s : iProp Σ :=
     (∃ vs, proph p vs ∗
-      ((not_done_state H l γ_h ∗
-        ( pending_state P n vs l_ghost γ_h γ_n
-        ∨ accepted_state Q vs l l_ghost γ_h ))
-      ∨ done_state Q l l_ghost γ_t γ_h))%I.
+      (own γ_s (Cinl $ Excl ()) ∗
+       (c_l ↦{1/2} #l ∗ ( pending_state P n (val_to_some_loc vs) l_ghost_winner γ_n
+        ∨ accepted_state Q (val_to_some_loc vs) l_ghost_winner ))
+       ∨ own γ_s (Cinr $ to_agree ()) ∗ done_state Q l l_ghost_winner γ_t))%I.
 
   Definition pau P Q γs :=
     (▷ P -∗ ◇ AU << ∀ (b : bool) (n : Z), counter_content γs (b, n) >> @ ⊤∖↑N, ∅
                  << counter_content γs (b, (if b then n + 1 else n)), COMM Q >>)%I.
 
-  Definition counter_inv γ_h γ_b γ_n f c :=
-    (∃ (b : bool) (l : loc) (H : list loc) (q : Qp) (v : val),
-       f ↦ #b ∗ c ↦ #l ∗ l ↦{q} v ∗
-       own γ_h (full_history_auth H) ∗
-       own γ_h (half_history_frag H) ∗
-       ([∗ list] l ∈ H, ∃ q, l ↦{q} -) ∗
-       ⌜Some l = head H ∧ NoDup H⌝ ∗
+  Definition counter_inv γ_b γ_n f c :=
+    (∃ (b : bool) (l : loc) (q : Qp) (s : abstract_state),
+       f ↦ #b ∗ c ↦{1/2} #l ∗ l ↦{q} (state_to_val s) ∗
        own γ_b (● Excl' b) ∗
-       ((∃ (n : Z), ⌜v = InjLV #n⌝ ∗ own γ_h (half_history_frag H) ∗ own γ_n (● Excl' n)) ∨
-        (∃ (n : Z) (p : proph_id), ⌜v = InjRV(#n,#p)⌝ ∗
-         ∃ P Q l_ghost γ_t, inv stateN (state_inv P Q p n l l_ghost H γ_h γ_n γ_t) ∗
-                    □ pau P Q (γ_h, γ_b, γ_n))))%I.
+       loc_token l ∗ (* the "location" token for ABA protection; also see [done_state] *)
+       match s with
+        | injl n => c ↦{1/2} #l ∗ own γ_n (● Excl' n)
+        | injr n p =>
+           ∃ P Q l_ghost_winner γ_t γ_s,
+             (* There are two pieces of per-[state]-protocol ghost state:
+             - [γ_t] is a token owned by whoever created this protocol and used
+               to get out the [Q] in the end.
+             - [γ_s] reflects whether the protocol is [done] yet or not. *)
+             inv stateN (state_inv P Q p n c l l_ghost_winner γ_n γ_t γ_s) ∗
+             □ pau P Q (γ_b, γ_n)
+       end)%I.
 
-  Definition is_counter (γs : gname * gname * gname) (ctr : val) :=
-    (∃ (γ_h γ_b γ_n : gname) (f c : loc),
-        ⌜γs = (γ_h, γ_b, γ_n) ∧ ctr = (#f, #c)%V⌝ ∗
-        inv counterN (counter_inv γ_h γ_b γ_n f c))%I.
+  Definition is_counter (γs : gname * gname) (ctr : val) :=
+    (∃ (γ_b γ_n : gname) (f c : loc),
+        ⌜γs = (γ_b, γ_n) ∧ ctr = (#f, #c)%V⌝ ∗
+        inv counterN (counter_inv γ_b γ_n f c))%I.
 
   Global Instance is_counter_persistent γs ctr : Persistent (is_counter γs ctr) := _.
 
@@ -540,233 +265,193 @@ Section conditional_counter.
     apply (iffLR (frac_valid' _)) in Hv. by apply Qp_not_plus_q_ge_1 in Hv.
   Qed.
 
-  Instance in_dec (l : loc) H: Decision (In l H).
+  Lemma loc_token_exclusive l :
+    loc_token l -∗ loc_token l -∗ False.
   Proof.
-    induction H as [|a H IH].
-    - right. naive_solver.
-    - destruct (decide (l = a)).
-      + left. naive_solver.
-      + destruct IH; [ left | right]; naive_solver.
+    iIntros "Hl1 Hl2".
+    iDestruct "Hl1" as (γ1) "[Hm1 Ht1]".
+    iDestruct "Hl2" as (γ2) "[Hm2 Ht2]".
+    iDestruct (meta_agree with "Hm1 Hm2") as %->.
+    iDestruct (own_valid_2 with "Ht1 Ht2") as %Hcontra.
+    by inversion Hcontra.
   Qed.
 
-  Lemma nodup_fresh_loc l v H:
-    NoDup H → l ↦ v -∗ ([∗ list] l ∈ H, ∃ q, l ↦{q} -) -∗ ⌜NoDup (l :: H)⌝.
+  Lemma loc_token_alloc v :
+    {{{ True }}} ref v {{{ l, RET #l; l ↦ v ∗ loc_token l }}}.
   Proof.
-    intros Hd. iIntros "Hl Hls".
-    destruct (decide (In l H)) as [(x1 & x2 & ->)%in_split | Hn%NoDup_cons]; last done.
-    - destruct x1 as [|x1 x1s];
-        [ rewrite app_nil_l in Hd; rewrite app_nil_l; iDestruct "Hls" as "[Hl' _]" |
-          iDestruct "Hls" as "[_ [Hl' _]]" ];
-        iDestruct "Hl'" as (q v') "Hl'";
-        by iDestruct (mapsto_valid_3 with "Hl Hl'") as %?.
-    - by iPureIntro.
+    iIntros (Φ) "HT HΦ". iApply wp_fupd.
+    wp_apply (wp_alloc with "HT"). iIntros (l_new) "[Hl_new Hm_new]".
+    iMod (own_alloc (Excl ())) as (γ_l) "Htok"; first done.
+    iMod ((meta_set _ _ γ_l N) with "Hm_new") as "Hm"; first done.
+    iApply "HΦ". iFrame "Hl_new". iExists _. by iFrame.
   Qed.
 
+  (** Once a [state] protocol is [done] (as reflected by the [γ_s] token here),
+      we can at any later point in time extract the [Q]. *)
+  Lemma state_done_extract_Q P Q p m c_l l l_ghost γ_n γ_t γ_s :
+    inv stateN (state_inv P Q p m c_l l l_ghost γ_n γ_t γ_s) -∗
+    own γ_s (Cinr (to_agree ())) -∗
+    □(own_token γ_t ={⊤}=∗ ▷ Q).
+  Proof.
+    iIntros "#Hinv #Hs !# Ht".
+    iInv stateN as (vs) "(Hp & [NotDone | Done])".
+    * (* Moved back to NotDone: contradiction. *)
+      iDestruct "NotDone" as "(>Hs' & _ & _)".
+      iDestruct (own_valid_2 with "Hs Hs'") as %?. contradiction.
+    * iDestruct "Done" as "(_ & QT & Hghost)".
+      iDestruct "QT" as "[Q | >T]"; last first.
+      { iDestruct (own_valid_2 with "Ht T") as %Contra.
+          by inversion Contra. }
+      iSplitR "Q"; last done. iIntros "!> !>". unfold state_inv.
+      iExists _. iFrame "Hp". iRight.
+      unfold done_state. iFrame "#∗".
+  Qed.
 
   (** ** Proof of [complete] *)
 
-  (** The part of [complete] for the succeeding thread that moves from [pending] to [accepted] state *)
-
-  Lemma complete_succeeding_thread_pending γ_h γ_b γ_n γ_t f_l c_l P Q p (m n : Z) l l_ghost l_new H Φ :
-    Some l = head H →
-    inv counterN (counter_inv γ_h γ_b γ_n f_l c_l) -∗
-    inv stateN (state_inv P Q p m l l_ghost H γ_h γ_n γ_t) -∗
-    pau P Q (γ_h, γ_b, γ_n) -∗
+  (** The part of [complete] for the succeeding thread that moves from [accepted] to [done] state *)
+  Lemma complete_succeeding_thread_pending (γ_b γ_n γ_t γ_s : gname) f_l c_l P Q p
+        (m n : Z) (l l_ghost l_new : loc) Φ :
+    inv counterN (counter_inv γ_b γ_n f_l c_l) -∗
+    inv stateN (state_inv P Q p m c_l l l_ghost γ_n γ_t γ_s) -∗
+    pau P Q (γ_b, γ_n) -∗
     l_ghost ↦{1 / 2} #() -∗
-    ((own_token γ_t ={⊤}=∗ ▷ Q) -∗ Φ #()) -∗
+    (□(own_token γ_t ={⊤}=∗ ▷ Q) -∗ Φ #()) -∗
     own γ_n (● Excl' n) -∗
     l_new ↦ InjLV #n -∗
+    loc_token l_new -∗
     WP Resolve (CAS #c_l #l #l_new) #p #l_ghost ;; #() {{ v, Φ v }}.
   Proof.
-    iIntros (Heq) "#InvC #InvS PAU Hl_ghost HQ Hn● Hl_new". wp_bind (Resolve _ _ _)%E.
-    iInv counterN as (b' l' H' q v) "[>Hf [>Hc [>Hl' [>H● [>H◯ [>HlH [>Heq [Hb● Hrest]]]]]]]]".
-    iDestruct "Heq" as %[Heq'' Hd']. simpl.
-    iDestruct ((nodup_fresh_loc _ _ _ Hd') with "Hl_new HlH") as %Hd''.
-    (* It must be that l' = l because we are in the succeeding thread. *)
-    destruct (decide (l' = l)) as [->|HNeq]; last first. {
-      iInv stateN as (vs') "[>Hp' [[>[Hh◯ _] State] | Done]]".
-      - iDestruct "State" as "[Pending | Accepted]".
-        + iDestruct "Pending" as "[_ >[_ Hn●']]".
-          iCombine "Hn●'" "Hn●" as "Contra".
-          iDestruct (own_valid with "Contra") as %Contra. by inversion Contra.
-        + iDestruct (sync_histories with "Hh◯ H◯") as %->.
-          rewrite <- Heq'' in Heq. by inversion Heq.
-      - iDestruct "Done" as "[_ >[Hlghost _]]".
-        wp_apply (wp_resolve with "Hp'"); first done. wp_cas_fail.
-        iDestruct "Hlghost" as (?) "Hlghost".
-        by iDestruct (mapsto_valid_2 with "Hlghost Hl_ghost") as %?.
-    }
-    (* To apply the CAS, we need the prophecy variable, so we open the state invariant. *)
-    iInv stateN as (vs') "[>Hp' [[>[Hh◯ Heq'] State] | Done]]".
-      - iDestruct "State" as "[Pending | Accepted]".
-        + (* Pending: contradiction. *)
-          iDestruct "Pending" as "[_ >[_ Hn●']]".
-          iCombine "Hn●" "Hn●'" as "Contra".
-          iDestruct (own_valid with "Contra") as %Contra. by inversion Contra.
-        + (* We perform the CAS. *)
-          iDestruct (sync_histories with "H◯ Hh◯") as %->.
-          wp_apply (wp_resolve with "Hp'"); first done; wp_cas_suc.
-          destruct (val_to_some_loc vs') eqn:Hvtsl; last first. {
-            (* Wrong prophecy: contradiction. *)
-            iIntros (vs ->). inversion Hvtsl.
-          }
-          (* Update to Done. *)
-          iDestruct "Accepted" as "[Hl_ghost_inv H]".
-          rewrite Hvtsl. iDestruct "H" as "[HEq Q]".
-          (* The first element of H is l. *)
-          destruct H as [|l' H]; inversion Heq; subst l'.
-          (* And we have l ≠ l_new. *)
-          destruct (decide (l = l_new)) as [->|HNeq]. {
-            iDestruct "HlH" as "[Hl HlH]". iDestruct "Hl" as (q' v') "Hl".
-            by iDestruct (mapsto_valid_3 with "Hl_new Hl") as %Contra.
-          }
-          (* Update histories. *)
-          iDestruct (update_history _ _ l_new with "H● H◯ Hh◯") as ">[Hh● [H◯ H◯']]".
-          iIntros (pv' ->) "Hp". iModIntro.
-          (* Extract snapshot to prove used_up. *)
-          iDestruct (extract_snapshot with "H◯'") as "#Hs".
-          iSplitL "Hl_ghost_inv Hl_ghost Q Hp".
-          (* Update state to Done. *)
-          { iNext. iExists _. iSplitL "Hp"; first done. repeat iRight.
-            iDestruct "Hl_ghost_inv" as (v'') "Hl_ghost''".
-            iDestruct (mapsto_agree with "Hl_ghost Hl_ghost''") as %<-.
-            iCombine "Hl_ghost" "Hl_ghost''" as "Hl_ghost'".
-            iSplitL "Q"; first by iFrame. iSplitL "Hl_ghost'"; first by eauto.
-            iExists (l_new :: l :: H). iSplit; first done. iPureIntro.
-            split; first by apply in_cons, in_eq. by intros [=->]. }
-          iModIntro. iSplitR "HQ".
-          { iNext. iExists _, _, _, _, _. iSplitL "Hf"; first done.
-            iSplitL "Hc"; first done. iDestruct "Hl_new" as "[$ Hl_new]".
-            iSplitL "Hh●"; first done. iSplitL "H◯'"; first done.
-            iSplitL "HlH Hl_new". { iSplitL "Hl_new"; first by iExists _, _. iFrame. }
-            iSplit; first done. iSplitL "Hb●"; first done. iLeft. iExists n. by iFrame. }
-          iApply wp_fupd. wp_seq. iApply "HQ". iModIntro. iIntros "Ht".
-          iInv stateN as (vs') "[>Hp' [[>[Hh◯ Heq'] _] | Done]]".
-          * iInv counterN as (b5 l5 H5 q5 v5) "[>Hf [>Hc [>Hl [>H● [>H◯ _]]]]]".
-            iDestruct (sync_histories with "H◯ Hh◯") as %->.
-            by iDestruct (sync_snapshot with "H● Hs") as %?%suffix_cons_not.
-          * iDestruct "Done" as "[QT [>Hlghost Usedup]]".
-            iModIntro. iDestruct (later_intro with "Ht") as "Ht".
-            iDestruct (later_or with "QT") as "[Q | T]"; last first.
-            { iCombine "Ht" "T" as "Contra". iDestruct (own_valid with "Contra") as "#Contra'".
-              iSplitL; try iModIntro; try iNext; iDestruct "Contra'" as %Contra;
-              by inversion Contra. }
-            iSplitR "Q"; last done. iNext. iExists _. iSplitL "Hp'"; first done.
-            repeat iRight. iFrame.
-      - (* Done: contradiction. *)
-        iDestruct "Done" as "[QT [>Hlghost Usedup]]".
-        iDestruct "Hlghost" as (v') "Hlghost".
+    iIntros "#InvC #InvS PAU Hl_ghost HQ Hn● Hlntok Hl_new". wp_bind (Resolve _ _ _)%E.
+    iInv counterN as (b' l' q s) "(>Hf & >Hc & >Hl' & Hb● & Hltok & Hrest)".
+    iInv stateN as (vs) "(>Hp & [NotDone | Done])"; last first.
+    { (* We cannot be [done] yet, as we own the "ghost location" that serves
+         as token for that transition. *)
+      iDestruct "Done" as "(_ & _ & Hlghost & _)".
+      iDestruct "Hlghost" as (v') ">Hlghost".
         by iDestruct (mapsto_valid_2 with "Hl_ghost Hlghost") as %?.
+    }
+    iDestruct "NotDone" as "(>Hs & >Hc' & [Pending | Accepted])".
+    { (* We also cannot be [Pending] any more we have [own γ_n] showing that this
+       transition has happened   *)
+       iDestruct "Pending" as "[_ >[_ Hn●']]".
+       iCombine "Hn●" "Hn●'" as "Contra".
+       iDestruct (own_valid with "Contra") as %Contra. by inversion Contra.
+    }
+    (* So, we are [Accepted]. Now we can show that l = l', because
+       while a [state] protocol is not [done], it owns enough of
+       the [counter] protocol to ensure that does not move anywhere else. *)
+    iDestruct (mapsto_agree with "Hc Hc'") as %[= ->].
+    (* We perform the CAS. *)
+    iCombine "Hc Hc'" as "Hc".
+    wp_apply (wp_resolve with "Hp"); first done; wp_cas_suc.
+    iIntros (vs' ->) "Hp'". simpl.
+    (* Update to Done. *)
+    iDestruct "Accepted" as "[Hl_ghost_inv [HEq Q]]".
+    iMod (own_update with "Hs") as "Hs".
+    { apply (cmra_update_exclusive (Cinr (to_agree ()))). done. }
+    iDestruct "Hs" as "#Hs'". iModIntro.
+    iSplitL "Hl_ghost_inv Hl_ghost Q Hltok Hp'".
+    (* Update state to Done. *)
+    { iNext. iExists _. iFrame "Hp'". iRight. unfold done_state.
+      iFrame "#∗". iExists _. done. }
+    iModIntro. iSplitR "HQ".
+    { iNext. iDestruct "Hc" as "[Hc1 Hc2]".
+      iExists _, l_new, _, (injl n). iFrame. }
+    iApply wp_fupd. wp_seq. iApply "HQ".
+    iApply state_done_extract_Q; done.
   Qed.
 
   (** The part of [complete] for the failing thread *)
-
-  Lemma complete_failing_thread γ_h γ_b γ_n γ_t f_l c_l l1 l H1 H P Q p m n l_ghost_inv l_ghost l_new Φ :
-    Some l1 = head H1 →
-    In l H1 →
+  Lemma complete_failing_thread γ_b γ_n γ_t γ_s f_l c_l l P Q p m n l_ghost_inv l_ghost l_new Φ :
     l_ghost_inv ≠ l_ghost →
-    inv counterN (counter_inv γ_h γ_b γ_n f_l c_l) -∗
-    inv stateN (state_inv P Q p m l l_ghost_inv H γ_h γ_n γ_t) -∗
-    pau P Q (γ_h, γ_b, γ_n) -∗
-    □ own γ_h (hist_snapshot H1) -∗
-    ((own_token γ_t ={⊤}=∗ ▷ Q) -∗ Φ #()) -∗
+    inv counterN (counter_inv γ_b γ_n f_l c_l) -∗
+    inv stateN (state_inv P Q p m c_l l l_ghost_inv γ_n γ_t γ_s) -∗
+    pau P Q (γ_b, γ_n) -∗
+    (□(own_token γ_t ={⊤}=∗ ▷ Q) -∗ Φ #()) -∗
     l_new ↦ InjLV #n -∗
     WP Resolve (CAS #c_l #l #l_new) #p #l_ghost ;; #() {{ v, Φ v }}.
   Proof.
-    iIntros (Heq Hin Hnl) "#InvC #InvS PAU #Hs1 HQ Hl_new". wp_bind (Resolve _ _ _)%E.
-    iInv counterN as (b l' H' q v) "[>Hf [>Hc [>Hl [>H● [>H◯ [HlH [>Heq [Hb● Hrest]]]]]]]]".
-    iDestruct (extract_snapshot with "H◯") as "#Hs2".
-    iDestruct (sync_snapshot with "H● Hs1") as %H12.
-    (* It must be that l' = l because we are in the succeeding thread. *)
-    destruct (decide (l' = l)) as [->|Hn]. {
-      iInv stateN as (vs') "[>Hp' [[>[Hh◯ _] State] | Done]]".
-      - wp_apply (wp_resolve with "Hp'"); first done; wp_cas_suc. iIntros (vs ->).
-        iDestruct "State" as "[Pending | Accepted]".
+    iIntros (Hnl) "#InvC #InvS PAU HQ Hl_new". wp_bind (Resolve _ _ _)%E.
+    iInv counterN as (b' l' q s) "(>Hf & >Hc & >Hl' & >Hb● & >Hltok & Hrest)".
+    iInv stateN as (vs) "(>Hp & [NotDone | [#Hs Done]])".
+    { (* If the [state] protocol is not done yet, we can show that it
+         is the active protocol still (l = l').  But then the CAS would
+         succeed, and our prophecy would have told us that.
+         So here we can prove that the prophecy was wrong. *)
+        iDestruct "NotDone" as "(_ & >Hc' & State)".
+        iDestruct (mapsto_agree with "Hc Hc'") as %[=->].
+        iCombine "Hc Hc'" as "Hc".
+        wp_apply (wp_resolve with "Hp"); first done; wp_cas_suc.
+        iIntros (vs' ->). iDestruct "State" as "[Pending | Accepted]".
         + iDestruct "Pending" as "[_ [Hvs _]]". iDestruct "Hvs" as %Hvs. by inversion Hvs.
-        + iDestruct "Accepted" as "[_ [Hvs _]]". iDestruct "Hvs" as %Hvs. by inversion Hvs.
-      - iDestruct "Done" as "[QT [>Hlghost Usedup]]".
-        iDestruct "Usedup" as (H'') "[Hs >Usedup]".
-        iDestruct "Usedup" as %[Hin' Hn].
-        iDestruct "Heq" as %[Heq' Hd'].
-        iMod (intuitionistically_elim with "Hs") as "Hs".
-        iDestruct (sync_snapshot with "H● Hs") as %Hs'.
-        destruct Hs' as [xs ->]. destruct (in_split _ _ Hin) as (x & y & ->).
-        destruct xs as [|z zs]; first done.
-        simpl in *. inversion Heq'; subst. destruct (in_split _ _ Hin') as (x1 & x2 & ->).
-        rewrite app_comm_cons in Hd'. rewrite app_assoc in Hd'.
-        apply (NoDup_remove _ _ _) in Hd' as [_ Contra].
-        rewrite <- app_comm_cons in Contra. simpl in *. exfalso. eauto.
+        + iDestruct "Accepted" as "[_ [Hvs _]]". iDestruct "Hvs" as %Hvs. by inversion Hvs. }
+    (* So, we know our protocol is [Done]. *)
+    (* It must be that l' ≠ l because we are in the failing thread. *)
+    destruct (decide (l' = l)) as [->|Hn]. {
+      (* The [state] protocol is [done] while still being the active protocol
+         of the [counter]?  Impossible, we got the location token for that! *)
+      iDestruct "Done" as "(_ & _ & >Hltok')".
+      iDestruct (loc_token_exclusive with "Hltok Hltok'") as "[]".
     }
     (* The CAS fails. *)
-    iInv stateN as (vs') "[>Hp' State]".
-    wp_apply (wp_resolve with "Hp'"); first done. wp_cas_fail.
-    iDestruct (extract_snapshot with "H◯") as "#Hs".
-    iIntros (vs ->) "Hp". iModIntro. iDestruct "Heq" as %[Heq' Hd'].
-    iSplitL "State Hp". { iNext. iExists vs. iFrame. } iModIntro.
-    iSplitL "Hf Hc Hl H● H◯ HlH Hb● Hrest". { iNext. iExists _, _, _, _. eauto with iFrame. }
-    wp_seq. iApply "HQ". iIntros "Ht".
-    iInv counterN as (b3 l3 H3 q3 v3) "[>Hf [>Hc [>Hl [>H● [>H◯ [HlH [>Heq [Hb● Hrest]]]]]]]]".
-    iDestruct "Heq" as %[Heq'' Hd''].
-    iInv stateN as (vs') "[>Hp' [[>[Hh◯ Heq'] _] | Done]]".
-    - iDestruct (sync_histories with "H◯ Hh◯") as %->.
-      iDestruct (sync_snapshot with "H● Hs") as %Hs.
-      iDestruct "Heq'" as %Heq'''. rewrite <- Heq'' in Heq'''.
-      inversion Heq'''. subst. exfalso.
-      by eapply (nodup_suffix_contradiction _ _ _ _ _ _ Heq Heq' Heq'').
-    - iDestruct "Done" as "[[Q | >T] Hrest']"; iModIntro.
-      + iSplitL "Ht Hp' Hrest'".
-        { iNext. iExists _. iSplitL "Hp'"; first done. repeat iRight. iFrame. }
-        iModIntro. iSplitR "Q"; last done. iNext. iExists _, _, _, _. eauto with iFrame.
-      + iCombine "T" "Ht" as "Contra".
-        iDestruct (own_valid with "Contra") as %Contra. by inversion Contra.
+    wp_apply (wp_resolve with "Hp"); first done. wp_cas_fail.
+    iIntros (vs' ->) "Hp". iModIntro.
+    iSplitL "Done Hp". { iNext. iExists _. iFrame "#∗". } iModIntro.
+    iSplitL "Hf Hc Hb● Hrest Hl' Hltok". { iNext. iExists _, _, _, _. iFrame. }
+    wp_seq. iApply "HQ".
+    iApply state_done_extract_Q; done.
   Qed.
 
   (** ** Proof of [complete] *)
-
-  Lemma complete_spec (c f l : loc) H (n : Z) (p : proph_id) γs γ_t l_ghost_inv P Q :
+  (* The postcondition basically says that *if* you were the thread to own
+     this request, then you get [Q].  But we also try to complete other
+     thread's requests, which is why we cannot ask for the token
+     as a precondition. *)
+  Lemma complete_spec (c f l : loc) (n : Z) (p : proph_id) γs γ_t γ_s l_ghost_inv P Q :
     is_counter γs (#f, #c) -∗
-    inv stateN (state_inv P Q p n l l_ghost_inv H γs.1.1 γs.2 γ_t) -∗
+    inv stateN (state_inv P Q p n c l l_ghost_inv γs.2 γ_t γ_s) -∗
     □ pau P Q γs -∗
     {{{ True }}}
        complete #c #f #l #n #p
-    {{{ RET #(); own_token γ_t ={⊤}=∗ ▷Q }}}.
+    {{{ RET #(); □ (own_token γ_t ={⊤}=∗ ▷Q) }}}.
   Proof.
-    iIntros "#InvC #InvS #PAU". destruct γs as [[γ_h γ_b] γ_n].
-    iDestruct "InvC" as (??? f_l c_l [[=<-<-<-][=->->]]) "#InvC".
+    iIntros "#InvC #InvS #PAU". destruct γs as [γ_b γ_n].
+    iDestruct "InvC" as (?? f_l c_l [[=<-<-][=->->]]) "#InvC".
     iModIntro. iIntros (Φ) "_ HQ". wp_lam. wp_pures.
     wp_alloc l_ghost as "[Hl_ghost' Hl_ghost'2]". wp_bind (! _)%E. simpl.
     (* open outer invariant to read `f` *)
-    iInv counterN as (b1 l1 H1 q1 v1) "[>Hf [>Hc [>Hl [>H● [>H◯ [Hlh1 [>Heq [Hb● Hrest]]]]]]]]".
-    iDestruct "Heq" as %[Heq Hd]. wp_load.
+    iInv counterN as (b' l' q s) "(>Hf & >Hc & >Hl' & >Hb● & >Hltok & Hrest)".
+    wp_load.
     (* two different proofs depending on whether we are succeeding thread *)
     destruct (decide (l_ghost_inv = l_ghost)) as [-> | Hnl].
     - (* we are the succeeding thread *)
-      (* we need to move from pending to accepted. *)
-      iInv stateN as (vs') "[>Hp' [[>[Hh◯ Heq] [Pending | Accepted]] | Done]]".
+      (* we need to move from [pending] to [accepted]. *)
+      iInv stateN as (vs) "(>Hp & [(>Hs & >Hc' & [Pending | Accepted]) | [#Hs Done]])".
       + (* Pending: update to accepted *)
-        iDestruct "Pending" as "[P >[Hvs Hn●]]". iDestruct "Heq" as %Heq'.
+        iDestruct "Pending" as "[P >[Hvs Hn●]]".
         iDestruct ("PAU" with "P") as ">AU".
-        (* open AU, sync flag and counter *)
+        (* open and *COMMIT* AU, sync flag and counter *)
         iMod "AU" as (b2 n2) "[CC [_ Hclose]]".
         iDestruct "CC" as "[Hb◯ Hn◯]". simpl.
         iDestruct (sync_flag_values with "Hb● Hb◯") as %->.
         iDestruct (sync_counter_values with "Hn● Hn◯") as %->.
-        iDestruct (sync_histories with "H◯ Hh◯") as %->.
-        rewrite <- Heq in Heq'. inversion_clear Heq'; subst.
         iMod (update_counter_value _ _ _ (if b2 then n2 + 1 else n2) with "Hn● Hn◯")
           as "[Hn● Hn◯]".
         iMod ("Hclose" with "[Hn◯ Hb◯]") as "Q"; first by iFrame.
         (* close state inv *)
-        iModIntro. iSplitL "Q H◯ Hl_ghost' Hp' Hvs".
-        { iNext. iExists _. iSplitL "Hp'"; first done. iLeft.
-          iSplitL "H◯"; first by iFrame. iRight. iSplitL "Hl_ghost'"; first by iExists _.
-          destruct (val_to_some_loc vs') eqn:Hvts; iFrame. }
+        iModIntro. iSplitL "Q Hl_ghost' Hp Hvs Hs Hc'".
+        { iNext. iExists _. iFrame "Hp". iLeft. iFrame.
+          iRight. iSplitL "Hl_ghost'"; first by iExists _.
+          destruct (val_to_some_loc vs) eqn:Hvts; iFrame. }
         (* close outer inv *)
         iModIntro. iSplitR "Hl_ghost'2 HQ Hn●".
-        { iNext. iExists _, _, _, _, _. iFrame. done. }
-        destruct b2; wp_if; [ wp_op | .. ]; wp_alloc l_new as "Hl_new"; wp_pures;
-          iApply ((complete_succeeding_thread_pending _ _ _ _ _ _ _ _ _ _ _ _ _ _ _ _ Heq)
-                    with "InvC InvS PAU Hl_ghost'2 HQ Hn● Hl_new").
+        { iNext. iExists _, _, _, _. iFrame. done. }
+        destruct b2; wp_if; [ wp_op | .. ];
+        wp_apply (loc_token_alloc with "[//]"); iIntros (l_new) "[Hl_new Hm_new]";
+        wp_pures;
+          iApply (complete_succeeding_thread_pending
+                    with "InvC InvS PAU Hl_ghost'2 HQ Hn● Hl_new Hm_new").
       + (* Accepted: contradiction *)
         iDestruct "Accepted" as "[>Hl_ghost_inv _]".
         iDestruct "Hl_ghost_inv" as (v) "Hlghost".
@@ -778,32 +463,13 @@ Section conditional_counter.
         iCombine "Hl_ghost'" "Hl_ghost'2" as "Hl_ghost'".
         by iDestruct (mapsto_valid_2 with "Hlghost Hl_ghost'") as %?.
     - (* we are the failing thread *)
-      (* extract history and assert that it contains l *)
-      iDestruct (extract_snapshot with "H◯") as "#Hs1".
-      iAssert (|={⊤ ∖ ↑counterN}=> (⌜In l H1⌝ ∗ own γ_h (full_history_auth H1)))%I with "[H●]" as "Hin". {
-        iInv stateN as (vs') "[>Hp' [[>[Hh◯ Heq'] State] | Done]]".
-        - iDestruct (sync_snapshot with "H● Hh◯") as %Hs1. iDestruct "Heq'" as %Heq'.
-          iModIntro. iSplitR "H●".
-          { iNext. iExists _. iSplitL "Hp'"; first done. iLeft. iFrame. done. }
-          iModIntro. iFrame. iPureIntro. by eapply suffix_in_head.
-        - iDestruct "Done" as "[QT [>Hlghost Usedup]]".
-          iDestruct "Usedup" as (H') "[Hs >Usedup]". iDestruct "Usedup" as %[Hin Hn].
-          iMod (intuitionistically_elim with "Hs") as "Hs".
-          iDestruct (sync_snapshot with "H● Hs") as %Hs'.
-          iModIntro. iSplitR "H●".
-          { iNext. iExists _. iSplitL "Hp'"; first done. repeat iRight. iFrame.
-            iExists _. iSplit; last by iPureIntro. iDestruct "Hs" as "#Hs". iModIntro.
-            iApply "Hs". }
-          iModIntro. iSplit; last done.
-          iPureIntro. by eapply suffix_in.
-      }
       (* close invariant *)
-      iMod "Hin" as (Hin) "H●". iModIntro.
-      iSplitL "Hf Hc H● H◯ Hb● Hrest Hl Hlh1". { iNext. iExists _, _, _, _. eauto with iFrame. }
+      iModIntro.
+      iSplitL "Hf Hc Hrest Hl' Hb● Hltok". { iNext. iExists _, _, _, _. iFrame. }
       (* two equal proofs depending on value of b1 *)
-      destruct b1; wp_if; [ wp_op | ..]; wp_alloc Hl_new as "Hl_new"; wp_pures;
-        iApply ((complete_failing_thread _ _ _ _ _ _ _ _ _ _ _ _ _ _ _ _ _ _ _ Heq Hin Hnl)
-                  with "InvC InvS PAU Hs1 HQ Hl_new").
+      destruct b'; wp_if; [ wp_op | ..]; wp_alloc Hl_new as "Hl_new"; wp_pures;
+        iApply (complete_failing_thread
+                  with "InvC InvS PAU HQ Hl_new"); done.
   Qed.
 
   (** ** Proof of [cinc] *)
@@ -814,96 +480,84 @@ Section conditional_counter.
         cinc (f, c)%V @⊤∖↑N
     <<< counter_content γs (b, if b then n + 1 else n), RET #() >>>.
   Proof.
-    iIntros "#InvC". iDestruct "InvC" as (γ_h γ_b γ_n f_l c_l) "[Heq InvC]".
+    iIntros "#InvC". iDestruct "InvC" as (γ_b γ_n f_l c_l) "[Heq InvC]".
     iDestruct "Heq" as %[-> [=->->]]. iIntros (Φ) "AU". iLöb as "IH".
     wp_lam. wp_proj. wp_let. wp_proj. wp_let. wp_bind (!_)%E.
-    iInv counterN as (b' l' H' q v) "[>Hf [>Hc [>[Hl Hl'] [>H● [>H◯ [Hlh [>Heq [>Hb● Hv]]]]]]]]".
-    wp_load. simpl. iDestruct "Hv" as "[Hv|Hv]".
-    - iDestruct "Hv" as (n) "[% Hv]"; subst v.
-      iModIntro. iSplitR "Hl' AU".
-      { iModIntro. iExists _, _, _, (q/2)%Qp, (InjLV #n). eauto with iFrame. }
+    iInv counterN as (b' l' q s) "(>Hf & >Hc & >[Hl Hl'] & >Hb● & >Hltok & Hrest)".
+    wp_load. destruct s as [n|n p].
+    - iDestruct "Hrest" as "(Hc' & Hv)".
+      iModIntro. iSplitR "AU Hl".
+      { iModIntro. iExists _, _, (q/2)%Qp, (injl n). iFrame. }
       wp_let. wp_load. wp_match. wp_apply wp_new_proph; first done.
       iIntros (l_ghost p') "Hp'".
-      wp_let. wp_alloc ly as "Hly". wp_let. wp_bind (CAS _ _ _)%E.
-      (* open outer invariant to read c_l *)
-      iInv counterN as (b l'' H'' q' v') "[>Hf [>Hc [>Hl'2 [>H● [>H◯ [>Hlh [>Heq [Hb● Hrest]]]]]]]]".
-      iDestruct "Heq" as %[Heq Hd].
-      (* assert that ly is not in the history *)
-      iDestruct (extract_snapshot with "H◯") as "#Hs".
-      iDestruct ((nodup_fresh_loc _ _ _ Hd) with "Hly Hlh") as %Hd'.
+      wp_let. wp_apply (loc_token_alloc with "[//]"); iIntros (ly) "[Hly Hmy]".
+      wp_let. wp_bind (CAS _ _ _)%E.
+      (* open outer invariant again to CAS c_l *)
+      iInv counterN as (b2 l'' q2 s) "(>Hf & >Hc & >Hl' & >Hb● & >Hltok & Hrest)".
       destruct (decide (l' = l'')) as [<- | Hn].
       + (* CAS succeeds *)
-        wp_cas_suc.
-        (* We need to update the half history with `ly`.
-           For that we will need to get the second half of the history *)
-        iDestruct "Hrest" as "[InjL | InjR]";
-          iPoseProof (mapsto_agree with "Hl' Hl'2") as "#Heq"; last first.
-        { (* injR: contradiction *)
-          iDestruct "InjR" as (??) "[Heq' InjR_rest]".
-          iDestruct "Heq'" as %->. iDestruct "Heq" as %Heq'. inversion Heq'. }
-        (* injL: update history *)
-        iDestruct "InjL" as (n'') "[Heq' [H◯' Hn●]]".
-        iDestruct "Heq'" as %->. simpl. iDestruct "Heq" as %[=<-].
-        iPoseProof ((update_history _ _ ly) with "H● H◯ H◯'") as ">[H● [H◯' H◯'']]".
+        iDestruct (mapsto_agree with "Hl Hl'") as %<-%state_to_val_inj.
+        iDestruct "Hrest" as ">[Hc' Hn●]". iCombine "Hc Hc'" as "Hc".
+        wp_cas_suc. iClear "Hltok".
+        (* Initialize new [state] protocol .*)
         iDestruct (laterable with "AU") as (AU_later) "[AU #AU_back]".
-        iDestruct (own_alloc token) as ">Ht"; first by apply auth_auth_valid.
-        iDestruct "Ht" as (γ_t) "Token".
+        iMod (own_alloc (Excl ())) as (γ_t) "Token"; first done.
+        iMod (own_alloc (Cinl $ Excl ())) as (γ_s) "Hs"; first done.
+        iDestruct "Hc" as "[Hc Hc']".
+        (* FIXME: This is three times almost the same thing to allocate the
+           invariant etc, it should be possible to deduplicate that. *)
         destruct (val_to_some_loc l_ghost) eqn:H.
         * destruct (val_to_some_loc_some l_ghost l H) as [v1 [v2 [vs' [-> HCases]]]].
           destruct HCases as [[-> ->] | Hl].
-          ++ iMod (inv_alloc stateN _ (state_inv AU_later _ _ _ _ _ _ _ _ γ_t)
-               with "[AU H◯' Hp' Hn●]") as "#Hinv".
-             { iNext. iExists _. iSplitL "Hp'"; first done. iLeft.
-               iSplitL "H◯'"; first by iFrame. iLeft. by iFrame. }
+          ++ iMod (inv_alloc stateN _ (state_inv AU_later _ _ _ _ _ _ _ _ _)
+               with "[AU Hs Hp' Hc' Hn●]") as "#Hinv".
+             { iNext. iExists _. iFrame "Hp'". iLeft. iFrame. iLeft.
+               iFrame. simpl. done. }
              iModIntro. iDestruct "Hly" as "[Hly1 Hly2]". iSplitR "Hl' Token". {
                (* close invariant *)
-               iNext. iExists _, ly, _, _, _. iFrame.
-               iSplitL "Hly1"; first by eauto. iSplit; first by iPureIntro.
-               iRight. iExists _, _. iSplit; first done. iExists _, _, _, _. iSplit; done.
+               iNext. iExists _, _, _, (injr n p'). iFrame.
+               iExists _, _, _, _, _. iSplit; done.
              }
-             wp_if.
-             wp_apply complete_spec; [iExists _, _, _, _, _; eauto | done | done | done | ..].
+             wp_if. wp_apply complete_spec; [iExists _, _, _, _; eauto | done | done | done | ..].
              iIntros "Ht". iMod ("Ht" with "Token") as "Φ". wp_seq. by wp_lam.
-          ++ iMod (inv_alloc stateN _ (state_inv AU_later _ _ _ ly l _ _ _ γ_t)
-               with "[AU H◯' Hp' Hn●]") as "#Hinv".
-             { iNext. iExists _. iSplitL "Hp'"; first done. iLeft.
-               iSplitL "H◯'"; first by iFrame. iLeft. iFrame. by rewrite H. }
+          ++ iMod (inv_alloc stateN _ (state_inv AU_later _ _ _ _ _ _ _ _ _)
+               with "[AU Hs Hp' Hc' Hn●]") as "#Hinv".
+             { iNext. iExists _. iSplitL "Hp'"; first done. iLeft. iFrame.
+               iLeft. iFrame. by rewrite H. }
              iModIntro. iDestruct "Hly" as "[Hly1 Hly2]". iSplitR "Hl' Token". {
                (* close invariant *)
-               iNext. iExists _, ly, _, _, _. iFrame.
-               iSplitL "Hly1"; first by eauto. iSplit; first by iPureIntro.
-               iRight. iExists _, _. iSplit; first done. iExists _, _, _, _. iSplit; done.
+               iNext. iExists _, _, _, (injr n p'). iFrame.
+               iExists _, _, _, _, _. iSplit; done.
              }
              wp_if.
-             wp_apply complete_spec; [iExists _, _, _, _, _; eauto | done | done | done | ..].
+             wp_apply complete_spec; [iExists _, _, _, _; eauto | done | done | done | ..].
              iIntros "Ht". iMod ("Ht" with "Token") as "Φ". wp_seq. by wp_lam.
-        * iMod (inv_alloc stateN _ (state_inv AU_later _ _ _ ly l' _ _ _ γ_t)
-            with "[AU H◯' Hp' Hn●]") as "#Hinv".
-          { iNext. iExists _. iSplitL "Hp'"; first done. iLeft.
-            iSplitL "H◯'"; first by iFrame. iLeft. iFrame. by rewrite H. }
+        * iMod (inv_alloc stateN _ (state_inv AU_later _ _ _ _ _ _ _ _ _)
+            with "[AU Hs Hp' Hc' Hn●]") as "#Hinv".
+          { iNext. iExists _. iSplitL "Hp'"; first done. iLeft. iFrame.
+            iLeft. iFrame. by rewrite H. }
           iModIntro. iDestruct "Hly" as "[Hly1 Hly2]". iSplitR "Hl' Token". {
             (* close invariant *)
-            iNext. iExists _, ly, _, _, _. iFrame.
-            iSplitL "Hly1"; first by eauto. iSplit; first by iPureIntro.
-            iRight. iExists _, _. iSplit; first done. iExists _, _, _, _. iSplit; done.
+            iNext. iExists _, _, _, (injr n p'). iFrame.
+            iExists _, _, ly, _, _. iSplit; done.
           }
           wp_if.
-          wp_apply complete_spec; [iExists _, _, _, _, _; eauto | done | done | done | ..].
+          wp_apply complete_spec; [iExists _, _, _, _; eauto | done | done | done | ..].
           iIntros "Ht". iMod ("Ht" with "Token") as "Φ". wp_seq. by wp_lam.
       + (* CAS fails: closing invariant and invoking IH *)
         wp_cas_fail.
-        iModIntro. iSplitR "Hl' AU".
-        iModIntro. iExists _, _, _, _. eauto 10 with iFrame.
+        iModIntro. iSplitR "AU".
+        { iModIntro. iExists _, _, _, s. iFrame. }
         wp_if. by iApply "IH".
     - (* l' ↦ injR *)
-      iModIntro. iDestruct "Hv" as (n p) "[% Hrest]"; subst v.
+      iModIntro.
       (* extract state invariant *)
-      iDestruct "Hrest" as (P Q l_ghost γ_t) "[#InvS #P_AU]".
+      iDestruct "Hrest" as (P Q l_ghost γ_t γ_s) "[#InvS #P_AU]".
       iSplitR "Hl' AU".
       (* close invariant *)
-      { iModIntro. iExists _, _, _, _, _. iFrame. iRight. eauto 10 with iFrame. }
-      wp_let. wp_load. wp_match. repeat wp_proj.
-      wp_apply complete_spec; [iExists _, _, _, _, _; eauto | done | done | done | ..].
+      { iModIntro. iExists _, _, _, (injr n p). iFrame. eauto 10 with iFrame. }
+      wp_let. wp_load. wp_match. wp_pures.
+      wp_apply complete_spec; [iExists _, _, _, _; eauto | done | done | done | ..].
       iIntros "_". wp_seq. by iApply "IH".
   Qed.
 
@@ -913,24 +567,20 @@ Section conditional_counter.
     {{{ ctr γs, RET ctr ; is_counter γs ctr ∗ counter_content γs (true, 0) }}}.
   Proof.
     iIntros (Φ) "_ HΦ". wp_lam. wp_apply wp_fupd.
-    wp_alloc l_n as "Hl_n". wp_alloc l_c as "Hl_c". wp_let.
+    wp_apply (loc_token_alloc with "[//]"); iIntros (l_n) "[Hl_n Hltok]".
+    wp_alloc l_c as "Hl_c". wp_let.
     wp_alloc l_f as "Hl_f". wp_let. wp_pair.
-    iMod (own_alloc (full_history_auth [l_n] ⋅ full_history_frag [l_n])) as (γ_h) "[Hh● Hh◯]".
-    { rewrite pair_op. apply pair_valid. split; by apply auth_both_valid. }
     iMod (own_alloc (● Excl' true  ⋅ ◯ Excl' true)) as (γ_b) "[Hb● Hb◯]".
     { by apply auth_both_valid. }
     iMod (own_alloc (● Excl' 0  ⋅ ◯ Excl' 0)) as (γ_n) "[Hn● Hn◯]".
     { by apply auth_both_valid. }
-    iMod (inv_alloc counterN _ (counter_inv γ_h γ_b γ_n l_f l_c)
-      with "[Hl_f Hl_c Hl_n Hh● Hh◯ Hb● Hn●]") as "#InvC".
-    { iNext. iDestruct "Hh◯" as "[Hh◯1 Hh◯2]". iDestruct "Hl_n" as "[Hl_n1 Hl_n2]".
-      iExists true, l_n, [l_n], _, (InjLV #0). iFrame.
-      iSplitL "Hl_n1". { simpl. iSplitL; last done. by iExists _, _. }
-      iSplitR. { iPureIntro. split; first done. apply NoDup_cons. apply in_nil. apply NoDup_nil. }
-      iLeft. iExists 0. iSplitR; first done. iFrame. }
+    iMod (inv_alloc counterN _ (counter_inv γ_b γ_n l_f l_c)
+      with "[Hl_f Hl_c Hl_n Hltok Hb● Hn●]") as "#InvC".
+    { iNext. iDestruct "Hl_c" as "[Hl_c1 Hl_c2]".
+      iExists true, l_n, _, (injl 0). iFrame. }
     iModIntro.
-    iApply ("HΦ" $! (#l_f, #l_c)%V (γ_h, γ_b, γ_n)).
-    iSplitR; last by iFrame. iExists γ_h, γ_b, γ_n, l_f, l_c. iSplit; done.
+    iApply ("HΦ" $! (#l_f, #l_c)%V (γ_b, γ_n)).
+    iSplitR; last by iFrame. iExists γ_b, γ_n, l_f, l_c. iSplit; done.
   Qed.
 
   Lemma set_flag_spec γs f c (new_b : bool) :
@@ -940,16 +590,16 @@ Section conditional_counter.
     <<< counter_content γs (new_b, n), RET #() >>>.
   Proof.
     iIntros "#InvC" (Φ) "AU". wp_lam. wp_let. wp_proj.
-    iDestruct "InvC" as (γ_h γ_b γ_n l_f l_c) "[[HEq1 HEq2] InvC]".
+    iDestruct "InvC" as (γ_b γ_n l_f l_c) "[[HEq1 HEq2] InvC]".
     iDestruct "HEq1" as %->. iDestruct "HEq2" as %HEq. inversion HEq; subst; clear HEq.
-    iInv counterN as (b c H q v) "[>Hl_f [>Hl_c [>Hl [>H● [>H◯ [>HlH [>HEq [Hb● H]]]]]]]]".
+    iInv counterN as (b c q s) "(>Hf & >Hc & >[Hl Hl'] & >Hb● & >Hltok & Hrest)".
     iMod "AU" as (b' n') "[[Hb◯ Hn◯] [_ Hclose]]"; simpl.
     wp_store.
     iDestruct (sync_flag_values with "Hb● Hb◯") as %HEq; subst b.
     iDestruct (update_flag_value with "Hb● Hb◯") as ">[Hb● Hb◯]".
     iMod ("Hclose" with "[Hn◯ Hb◯]") as "HΦ"; first by iFrame.
     iModIntro. iModIntro. iSplitR "HΦ"; last done.
-    iNext. iExists new_b, c, H, q, v. iFrame.
+    iNext. iExists new_b, c, q, _. iFrame. done.
   Qed.
 
   Lemma get_spec γs f c :
@@ -959,26 +609,26 @@ Section conditional_counter.
     <<< counter_content γs (b, n), RET #n >>>.
   Proof.
     iIntros "#InvC" (Φ) "AU". iLöb as "IH". wp_lam. repeat (wp_proj; wp_let). wp_bind (! _)%E.
-    iDestruct "InvC" as (γ_h γ_b γ_n l_f l_c) "[[HEq1 HEq2] InvC]".
+    iDestruct "InvC" as (γ_b γ_n l_f l_c) "[[HEq1 HEq2] InvC]".
     iDestruct "HEq1" as %->. iDestruct "HEq2" as %HEq. inversion HEq; subst.
-    iInv counterN as (b c H q v) "[>Hl_f [>Hl_c [>[Hc Hc'] [>H● [>H◯ [>HlH [>HEq [Hb● [H|H]]]]]]]]]".
-    - wp_load. iDestruct "H" as (n) "[% [H◯2 Hn●]]". simpl in *; subst v.
-      iMod "AU" as (au_b au_n) "[[Hb◯ Hn◯] [_ Hclose]]"; simpl.
+    iInv counterN as (b c q s) "(>Hf & >Hc & >[Hl Hl'] & >Hb● & >Hltok & Hrest)".
+    wp_load.
+    destruct s as [n|n p].
+    - iMod "AU" as (au_b au_n) "[[Hb◯ Hn◯] [_ Hclose]]"; simpl.
+      iDestruct "Hrest" as "[Hc' Hn●]".
       iDestruct (sync_counter_values with "Hn● Hn◯") as %->.
       iMod ("Hclose" with "[Hn◯ Hb◯]") as "HΦ"; first by iFrame.
-      iModIntro. iSplitR "HΦ Hc'". {
-        iNext. iExists b, c, H, (q/2)%Qp, (InjLV #au_n). iFrame.
-        iLeft. iExists au_n. iFrame. done.
+      iModIntro. iSplitR "HΦ Hl'". {
+        iNext. iExists b, c, (q/2)%Qp, (injl au_n). iFrame.
       }
       wp_let. wp_load. wp_match. iApply "HΦ".
-    - wp_load. iDestruct "H" as (n p) "[% H]". simpl in *; subst v.
-      iDestruct "H" as (P Q l_ghost γ_t) "[#InvS #PAU]".
-      iModIntro. iSplitR "AU Hc'". {
-        iNext. iExists b, c, H, (q/2)%Qp, (InjRV(#n,#p)). iFrame.
-        iRight. iExists n, p. iSplit; first done. iExists P, Q, l_ghost, γ_t. eauto.
+    - iDestruct "Hrest" as (P Q l_ghost γ_t γ_s) "[#InvS #PAU]".
+      iModIntro. iSplitR "AU Hl'". {
+        iNext. iExists b, c, (q/2)%Qp, (injr n p). iFrame.
+        iExists P, Q, l_ghost, γ_t, _. eauto.
       }
       wp_let. wp_load. wp_match. repeat wp_proj. wp_bind (complete _ _ _ _ _)%E.
-      wp_apply complete_spec; [ iExists _, _, _, _, _; eauto | done | done | done | .. ].
+      wp_apply complete_spec; [ iExists _, _, _, _; eauto | done | done | done | .. ].
       iIntros "Ht". wp_seq. iApply "IH". iApply "AU".
   Qed.
 
